finished adding parity and right shift to IMP- -> IMP--

IMP-_To_SAS+/IMP-_To_IMP--/Binary_Operations.thy
@@ -51,8 +51,7 @@ lemma com_list_to_seq_of_length_one_terminates_iff:
 lemma com_list_to_seq_variables: "set (enumerate_variables (com_list_to_seq cs))
   = { v | v c. c \<in> set cs \<and> v \<in> set (enumerate_variables c)}" 
   apply(induction cs)
-   apply(auto simp: set_enumerate_variables_seq)
-  by(simp add: enumerate_variables_def)
+  by(auto simp: set_enumerate_variables_seq)
 
 fun binary_assign_constant:: "nat \<Rightarrow> vname \<Rightarrow> nat \<Rightarrow> IMP_Minus_Minus_com" where 
 "binary_assign_constant 0 v x = SKIP" |
@@ -76,8 +75,7 @@ qed (auto simp: fun_eq_iff split: option.splits)
 lemma binary_assign_constant_variables: "set (enumerate_variables (binary_assign_constant n v x))
   = { var_bit_to_var (v, i) | i. i < n }" 
   apply(induction n)
-   apply(auto simp: set_enumerate_variables_seq)
-  by(auto simp: enumerate_variables_def)
+  by(auto simp: set_enumerate_variables_seq)
 
 lemma result_of_binary_assign_constant_on_translated_state_aux:
   assumes "n > 0"
@@ -463,10 +461,9 @@ lemma subtract_handle_underflow_variables:
   = { operand_bit_to_var (op, i) | i op. i < n \<and> (op = CHR ''a'' \<or> op = CHR ''b'') } 
     \<union> { var_bit_to_var (v, i) | i. i < n }
     \<union> { ''carry'' }"
-  apply(auto simp: subtract_handle_underflow_def 
+  by(auto simp: subtract_handle_underflow_def 
       set_enumerate_variables_seq com_list_to_seq_variables full_subtractor_variables
       set_enumerate_variables_if underflow_handler_def binary_assign_constant_variables)
-  by(auto simp: underflow_handler_def enumerate_variables_def split: if_splits)
 
 definition binary_subtractor:: "nat \<Rightarrow> vname \<Rightarrow> AExp.atomExp \<Rightarrow> AExp.atomExp \<Rightarrow> IMP_Minus_Minus_com" where
 "binary_subtractor n v a b = 
@@ -489,12 +486,17 @@ lemma binary_subtractor_correct:
   assms 
   by(fastforce simp: binary_subtractor_def IMP_Minus_State_To_IMP_Minus_Minus_def)
 
+text \<open> The two copy_atom_to_operand which don't have any effect on the output are only a hack to
+       ensure that all bits of all variables in IMP- occur in IMP-- \<close> 
+
 fun binary_parity:: "nat \<Rightarrow> vname \<Rightarrow> AExp.atomExp \<Rightarrow> IMP_Minus_Minus_com" where
 "binary_parity n v (N a) = binary_assign_constant n v (a mod 2)" |
-"binary_parity n v (V a) = IF [var_bit_to_var (a, 0)]\<noteq>0 THEN
+"binary_parity n v (V a) = (IF [var_bit_to_var (a, 0)]\<noteq>0 THEN
     binary_assign_constant n v 1
   ELSE
-    binary_assign_constant n v 0"
+    binary_assign_constant n v 0) ;;
+  (copy_atom_to_operand n (CHR ''a'') (AExp.V a) ;;
+  copy_atom_to_operand n (CHR ''a'') (AExp.N 0))"
 
 lemma binary_parity_correct:
   assumes "n > 0"
@@ -504,40 +506,130 @@ lemma binary_parity_correct:
   apply(cases a)
    apply simp
    apply(rule result_of_binary_assign_constant_on_translated_state[OF \<open>n > 0\<close>, simplified])
-  apply(auto simp: t_small_step_fun_terminate_iff)
-     apply(auto simp: t_small_step_fun_small_step_fun)
-  using t_small_step_fun_increase_time
-    [OF _ result_of_binary_assign_constant_on_translated_state_aux[OF \<open>n > 0\<close>]]
+  apply(simp add: IMP_Minus_State_To_IMP_Minus_Minus_def)
+  apply(subst seq_terminates_when
+      [OF _ _ seq_terminates_when[OF _ copy_atom_to_operand_a_result copy_atom_to_operand_a_result],
+        where ?t1.0="3 * n + 1" and ?t2.0="9 * n"])
+  using result_of_binary_assign_constant_on_translated_state_aux \<open>n > 0\<close>
   by(auto simp: IMP_Minus_State_To_IMP_Minus_Minus_def nth_bit_def nat_to_bit_eq_One_iff 
-      nat_to_bit_eq_Zero_iff split: if_splits)
+      t_small_step_fun_small_step_fun nat_to_bit_eq_Zero_iff split: if_splits)
+
+lemma binary_parity_variables: "n > 0 \<Longrightarrow> set (enumerate_variables (binary_parity n v a))
+  = { var_bit_to_var (v, i) | i. i < n } 
+    \<union> (case a of (V v') \<Rightarrow> 
+        { var_bit_to_var (v', i) | i. i < n } \<union> { operand_bit_to_var (CHR ''a'', i) | i. i < n } |
+        _ \<Rightarrow> ({}))"
+  apply(cases a)
+  by(auto simp: binary_assign_constant_variables copy_atom_to_operand_variables
+      var_bit_to_var_neq_operand_bit_to_var[symmetric]
+      set_enumerate_variables_seq set_enumerate_variables_if)
+
+fun assign_shifted_bits:: "nat \<Rightarrow> vname \<Rightarrow> IMP_Minus_Minus_com" where
+"assign_shifted_bits 0 v = SKIP" |
+"assign_shifted_bits (Suc i) v = (IF [operand_bit_to_var ((CHR ''a''), Suc i)]\<noteq>0 THEN 
+    (var_bit_to_var (v, i)) ::= One
+  ELSE
+    (var_bit_to_var (v, i)) ::= Zero) ;;
+  assign_shifted_bits i v"
+
+lemma result_of_assign_shifted_bits: 
+  "t_small_step_fun (3 * k) (assign_shifted_bits k v, s) = (SKIP, (\<lambda>w. 
+    (case var_to_var_bit w of Some(v', i) \<Rightarrow> (if v' = v \<and> i < k then 
+      (if s (operand_bit_to_var (CHR ''a'', Suc i)) \<noteq> Some Zero then Some One else Some Zero)
+      else s w) |
+      _ \<Rightarrow> s w)))"
+proof(induction k arbitrary: s)
+  case (Suc k)
+  have *: "t_small_step_fun 2 (IF [operand_bit_to_var ((CHR ''a''), Suc k)]\<noteq>0 THEN 
+      (var_bit_to_var (v, k)) ::= One
+   ELSE
+      (var_bit_to_var (v, k)) ::= Zero, s) = (SKIP, s(var_bit_to_var (v, k) \<mapsto> 
+        (if s (operand_bit_to_var (CHR ''a'', Suc k)) \<noteq> Some Zero then One else Zero)))" 
+    by(auto simp: numeral_2_eq_2)
+  show ?case 
+    using seq_terminates_when[OF _ * Suc.IH, where ?t="3 + 3 * k"]
+    apply (auto simp: fun_eq_iff var_to_var_bit_eq_Some_iff split: option.splits)
+    using var_bit_to_var_neq_operand_bit_to_var
+    by (metis operand_bit_to_var.simps)+
+qed (auto simp: fun_eq_iff split: option.splits)
+
+lemma assign_shifted_bits_variables: "set (enumerate_variables (assign_shifted_bits k v)) 
+  = { var_bit_to_var (v, i) | i. i < k } \<union> { operand_bit_to_var (CHR ''a'', i) | i. i > 0 \<and> i \<le> k }" 
+  apply(induction k)
+   apply(auto simp: set_enumerate_variables_seq set_enumerate_variables_if)
+  using operand_bit_to_var_eq_operand_bit_to_var_iff'
+  by (metis Suc_eq_plus1 le_SucE)
+
+definition assign_shifted_bits_and_zero_most_significant:: 
+  "nat \<Rightarrow> vname \<Rightarrow> IMP_Minus_Minus_com" where
+"assign_shifted_bits_and_zero_most_significant n v = assign_shifted_bits (n - 1) v ;;
+  (var_bit_to_var (v, n - 1)) ::= Zero" 
+
+lemma assign_shifted_bits_and_zero_most_significant_correct:
+  assumes "n > 0" "a < 2 ^ n" 
+  shows "t_small_step_fun (3 * n) (assign_shifted_bits_and_zero_most_significant n v, 
+    IMP_Minus_State_To_IMP_Minus_Minus_with_operands_a_b s n a b)
+    = (SKIP, IMP_Minus_State_To_IMP_Minus_Minus_with_operands_a_b (s(v := a div 2)) n a b)"
+  apply(simp only: assign_shifted_bits_and_zero_most_significant_def)
+  apply(rule seq_terminates_when[OF _ result_of_assign_shifted_bits, where ?t2.0=1])
+  using assms apply(auto simp: fun_eq_iff var_to_var_bit_eq_Some_iff div2_is_right_shift 
+      le_2_to_the_n_then_nth_bit_zero split: option.splits)
+  using IMP_Minus_State_To_IMP_Minus_Minus_with_operands_a_b_of_changed_s_neq_iff
+  by (metis option.simps)
+
+
+definition binary_right_shift:: "nat \<Rightarrow> vname \<Rightarrow> AExp.atomExp \<Rightarrow> IMP_Minus_Minus_com" where
+"binary_right_shift n v a =  copy_atom_to_operand n (CHR ''a'') a ;;
+    assign_shifted_bits_and_zero_most_significant n v ;;
+    copy_atom_to_operand n (CHR ''a'') (N 0)" 
+
+lemma binary_right_shift_correct:
+  assumes "n > 0" "atomVal a s < 2 ^ n" 
+  shows "t_small_step_fun (50 * (n + 1)) (binary_right_shift n v a, 
+  IMP_Minus_State_To_IMP_Minus_Minus s n) = 
+  (SKIP, IMP_Minus_State_To_IMP_Minus_Minus (s(v := atomVal a s div 2)) n)" 
+  apply(simp only: IMP_Minus_State_To_IMP_Minus_Minus_def binary_right_shift_def)
+  using seq_terminates_when[OF _ seq_terminates_when[OF _ copy_atom_to_operand_a_result 
+          assign_shifted_bits_and_zero_most_significant_correct] 
+        copy_atom_to_operand_a_result, where ?t1.0="8 * n"]
+  using assms by auto
 
 definition assignment_to_binary:: "nat \<Rightarrow> vname \<Rightarrow> AExp.aexp \<Rightarrow> IMP_Minus_Minus_com" where
 "assignment_to_binary n v aexp = (case aexp of
   AExp.A a \<Rightarrow> binary_adder n v a (AExp.N 0) |
   AExp.Plus a b \<Rightarrow> binary_adder n v a b |
-  AExp.Sub a b \<Rightarrow> binary_subtractor n v a b)" 
+  AExp.Sub a b \<Rightarrow> binary_subtractor n v a b |
+  AExp.Parity a \<Rightarrow> binary_parity n v a |
+  AExp.RightShift a \<Rightarrow> binary_right_shift n v a)" 
 
 lemma assignment_to_binary_correct: 
   assumes "n > 0"  "AExp.aval a s < 2 ^ n" "\<forall>v. s v < 2 ^ n" "aexp_max_constant a < 2 ^ n"
   shows "t_small_step_fun (50 * (n + 1)) (assignment_to_binary n v a,  
   IMP_Minus_State_To_IMP_Minus_Minus s n) 
   = (SKIP, IMP_Minus_State_To_IMP_Minus_Minus (s(v := AExp.aval a s)) n)" 
-using assms binary_adder_correct proof(cases a)
+using assms binary_adder_correct  proof(cases a)
   case (Sub x31 x32)
   then show ?thesis 
     apply(simp add: assignment_to_binary_def)  
     apply(rule binary_subtractor_correct[simplified])
     using assms by(cases x31; cases x32; auto)+
-qed (auto simp: assignment_to_binary_def)
+next
+  case (RightShift x5)
+  then show ?thesis using assms apply(simp add: assignment_to_binary_def)
+    apply(rule binary_right_shift_correct[simplified])
+    by (cases x5; auto)+
+qed (auto simp: assignment_to_binary_def binary_parity_correct[simplified])
 
 lemma assignment_to_binary_variables:
-  "set (enumerate_variables (assignment_to_binary n v a)) \<subseteq> 
+  "n > 0 \<Longrightarrow> set (enumerate_variables (assignment_to_binary n v a)) \<subseteq> 
     { var_bit_to_var (w, i) | w i. i < n \<and> (w = v \<or> w \<in> set (aexp_vars a)) }
     \<union> { operand_bit_to_var (op, i) | op i. i < n \<and> (op = CHR ''a'' \<or> op = CHR ''b'') }
     \<union> { ''carry'' }" 
   apply(cases a)
   by(auto simp: assignment_to_binary_def binary_adder_def set_enumerate_variables_seq 
       copy_atom_to_operand_variables adder_def com_list_to_seq_variables full_adder_variables
-    binary_subtractor_def subtract_handle_underflow_variables)
+    binary_subtractor_def subtract_handle_underflow_variables binary_parity_variables
+    binary_right_shift_def assign_shifted_bits_and_zero_most_significant_def 
+    assign_shifted_bits_variables split: atomExp.splits)
 
 end 
